Wasm/Text/Notation/Index.lean
@@ -11,19 +11,19 @@ scoped syntax wat_u32      : wat_index
 scoped syntax wat_ident    : wat_index
 scoped syntax "↑" term:max : wat_index
 
-scoped syntax "[wat_index|" wat_index "]"      : term
-scoped syntax "[wat_vec_index|" wat_index* "]" : term
+scoped syntax ">>wat_index|" wat_index "<<"      : term
+scoped syntax ">>wat_vec_index|" wat_index* "<<" : term
 
 macro_rules
-| `([wat_index| $x:wat_u32 ])    => `(Index.num [wat_u32| $x])
-| `([wat_index| $id:wat_ident ]) => `(Index.name [wat_ident| $id])
-| `([wat_index| ↑$e ])           => `(Index.name $e)
+| `(>>wat_index| $x:wat_u32 <<)    => `(Index.num >>wat_u32| $x<<)
+| `(>>wat_index| $id:wat_ident <<) => `(Index.name >>wat_ident| $id<<)
+| `(>>wat_index| ↑$e <<)           => `(Index.name $e)
 
 macro_rules
-| `([wat_vec_index| ]) => `(Vec.nil)
-| `([wat_vec_index| $i:wat_index]) => `(Vec.single [wat_index| $i])
-| `([wat_vec_index| $i:wat_index $is:wat_index*]) =>
-    `(Vec.cons [wat_index| $i] [wat_vec_index| $is*])
+| `(>>wat_vec_index| <<) => `(Vec.nil)
+| `(>>wat_vec_index| $i:wat_index<<) => `(Vec.single >>wat_index| $i<<)
+| `(>>wat_vec_index| $i:wat_index $is:wat_index*<<) =>
+    `(Vec.cons >>wat_index| $i<< >>wat_vec_index| $is*<<)
 
 
 /- Various indices -- these don't really matter since we check the context
@@ -50,80 +50,80 @@ scoped syntax wat_index : wat_dataidx
 scoped syntax wat_index : wat_localidx
 scoped syntax wat_index : wat_labelidx
 
-scoped syntax "[wat_typeidx|"   wat_typeidx   "]" : term
-scoped syntax "[wat_funcidx|"   wat_funcidx   "]" : term
-scoped syntax "[wat_tableidx|"  wat_tableidx  "]" : term
-scoped syntax "[wat_memidx|"    wat_memidx    "]" : term
-scoped syntax "[wat_globalidx|" wat_globalidx "]" : term
-scoped syntax "[wat_elemidx|"   wat_elemidx   "]" : term
-scoped syntax "[wat_dataidx|"   wat_dataidx   "]" : term
-scoped syntax "[wat_localidx|"  wat_localidx  "]" : term
-scoped syntax "[wat_labelidx|"  wat_labelidx  "]" : term
+scoped syntax ">>wat_typeidx|"   wat_typeidx   "<<" : term
+scoped syntax ">>wat_funcidx|"   wat_funcidx   "<<" : term
+scoped syntax ">>wat_tableidx|"  wat_tableidx  "<<" : term
+scoped syntax ">>wat_memidx|"    wat_memidx    "<<" : term
+scoped syntax ">>wat_globalidx|" wat_globalidx "<<" : term
+scoped syntax ">>wat_elemidx|"   wat_elemidx   "<<" : term
+scoped syntax ">>wat_dataidx|"   wat_dataidx   "<<" : term
+scoped syntax ">>wat_localidx|"  wat_localidx  "<<" : term
+scoped syntax ">>wat_labelidx|"  wat_labelidx  "<<" : term
 
-scoped syntax "[wat_vec_typeidx|"   wat_typeidx*   "]" : term
-scoped syntax "[wat_vec_funcidx|"   wat_funcidx*   "]" : term
-scoped syntax "[wat_vec_tableidx|"  wat_tableidx*  "]" : term
-scoped syntax "[wat_vec_memidx|"    wat_memidx*    "]" : term
-scoped syntax "[wat_vec_globalidx|" wat_globalidx* "]" : term
-scoped syntax "[wat_vec_elemidx|"   wat_elemidx*   "]" : term
-scoped syntax "[wat_vec_dataidx|"   wat_dataidx*   "]" : term
-scoped syntax "[wat_vec_localidx|"  wat_localidx*  "]" : term
-scoped syntax "[wat_vec_labelidx|"  wat_labelidx*  "]" : term
-
-macro_rules
-| `([wat_typeidx|   $i:wat_index ]) => `([wat_index| $i])
-| `([wat_funcidx|   $i:wat_index ]) => `([wat_index| $i])
-| `([wat_tableidx|  $i:wat_index ]) => `([wat_index| $i])
-| `([wat_memidx|    $i:wat_index ]) => `([wat_index| $i])
-| `([wat_globalidx| $i:wat_index ]) => `([wat_index| $i])
-| `([wat_elemidx|   $i:wat_index ]) => `([wat_index| $i])
-| `([wat_dataidx|   $i:wat_index ]) => `([wat_index| $i])
-| `([wat_localidx|  $i:wat_index ]) => `([wat_index| $i])
-| `([wat_labelidx|  $i:wat_index ]) => `([wat_index| $i])
+scoped syntax ">>wat_vec_typeidx|"   wat_typeidx*   "<<" : term
+scoped syntax ">>wat_vec_funcidx|"   wat_funcidx*   "<<" : term
+scoped syntax ">>wat_vec_tableidx|"  wat_tableidx*  "<<" : term
+scoped syntax ">>wat_vec_memidx|"    wat_memidx*    "<<" : term
+scoped syntax ">>wat_vec_globalidx|" wat_globalidx* "<<" : term
+scoped syntax ">>wat_vec_elemidx|"   wat_elemidx*   "<<" : term
+scoped syntax ">>wat_vec_dataidx|"   wat_dataidx*   "<<" : term
+scoped syntax ">>wat_vec_localidx|"  wat_localidx*  "<<" : term
+scoped syntax ">>wat_vec_labelidx|"  wat_labelidx*  "<<" : term
 
 macro_rules
-| `([wat_vec_typeidx|   $i:wat_typeidx   $is:wat_typeidx  * ]) =>
-    `(Vec.cons [wat_typeidx| $i]   [wat_vec_typeidx| $is*   ] sorry)
-| `([wat_vec_funcidx|   $i:wat_funcidx   $is:wat_funcidx  * ]) =>
-    `(Vec.cons [wat_funcidx| $i]   [wat_vec_funcidx| $is*   ] sorry)
-| `([wat_vec_tableidx|  $i:wat_tableidx  $is:wat_tableidx * ]) =>
-    `(Vec.cons [wat_tableidx| $i]  [wat_vec_tableidx| $is*  ] sorry)
-| `([wat_vec_memidx|    $i:wat_memidx    $is:wat_memidx   * ]) =>
-    `(Vec.cons [wat_memidx| $i]    [wat_vec_memidx| $is*    ] sorry)
-| `([wat_vec_globalidx| $i:wat_globalidx $is:wat_globalidx* ]) =>
-    `(Vec.cons [wat_globalidx| $i] [wat_vec_globalidx| $is* ] sorry)
-| `([wat_vec_elemidx|   $i:wat_elemidx   $is:wat_elemidx  * ]) =>
-    `(Vec.cons [wat_elemidx| $i]   [wat_vec_elemidx| $is*   ] sorry)
-| `([wat_vec_dataidx|   $i:wat_dataidx   $is:wat_dataidx  * ]) =>
-    `(Vec.cons [wat_dataidx| $i]   [wat_vec_dataidx| $is*   ] sorry)
-| `([wat_vec_localidx|  $i:wat_localidx  $is:wat_localidx * ]) =>
-    `(Vec.cons [wat_localidx| $i]  [wat_vec_localidx| $is*  ] sorry )
-| `([wat_vec_labelidx|  $i:wat_labelidx  $is:wat_labelidx * ]) =>
-    `(Vec.cons [wat_labelidx| $i]  [wat_vec_labelidx| $is*  ] sorry )
+| `(>>wat_typeidx|   $i:wat_index <<) => `(>>wat_index| $i<<)
+| `(>>wat_funcidx|   $i:wat_index <<) => `(>>wat_index| $i<<)
+| `(>>wat_tableidx|  $i:wat_index <<) => `(>>wat_index| $i<<)
+| `(>>wat_memidx|    $i:wat_index <<) => `(>>wat_index| $i<<)
+| `(>>wat_globalidx| $i:wat_index <<) => `(>>wat_index| $i<<)
+| `(>>wat_elemidx|   $i:wat_index <<) => `(>>wat_index| $i<<)
+| `(>>wat_dataidx|   $i:wat_index <<) => `(>>wat_index| $i<<)
+| `(>>wat_localidx|  $i:wat_index <<) => `(>>wat_index| $i<<)
+| `(>>wat_labelidx|  $i:wat_index <<) => `(>>wat_index| $i<<)
 
-| `([wat_vec_typeidx|   ]) => `(Vec.nil)
-| `([wat_vec_funcidx|   ]) => `(Vec.nil)
-| `([wat_vec_tableidx|  ]) => `(Vec.nil)
-| `([wat_vec_memidx|    ]) => `(Vec.nil)
-| `([wat_vec_globalidx| ]) => `(Vec.nil)
-| `([wat_vec_elemidx|   ]) => `(Vec.nil)
-| `([wat_vec_dataidx|   ]) => `(Vec.nil)
-| `([wat_vec_localidx|  ]) => `(Vec.nil)
-| `([wat_vec_labelidx|  ]) => `(Vec.nil)
+macro_rules
+| `(>>wat_vec_typeidx|   $i:wat_typeidx   $is:wat_typeidx  * <<) =>
+    `(Vec.cons >>wat_typeidx| $i<<   >>wat_vec_typeidx| $is*   << sorry)
+| `(>>wat_vec_funcidx|   $i:wat_funcidx   $is:wat_funcidx  * <<) =>
+    `(Vec.cons >>wat_funcidx| $i<<   >>wat_vec_funcidx| $is*   << sorry)
+| `(>>wat_vec_tableidx|  $i:wat_tableidx  $is:wat_tableidx * <<) =>
+    `(Vec.cons >>wat_tableidx| $i<<  >>wat_vec_tableidx| $is*  << sorry)
+| `(>>wat_vec_memidx|    $i:wat_memidx    $is:wat_memidx   * <<) =>
+    `(Vec.cons >>wat_memidx| $i<<    >>wat_vec_memidx| $is*    << sorry)
+| `(>>wat_vec_globalidx| $i:wat_globalidx $is:wat_globalidx* <<) =>
+    `(Vec.cons >>wat_globalidx| $i<< >>wat_vec_globalidx| $is* << sorry)
+| `(>>wat_vec_elemidx|   $i:wat_elemidx   $is:wat_elemidx  * <<) =>
+    `(Vec.cons >>wat_elemidx| $i<<   >>wat_vec_elemidx| $is*   << sorry)
+| `(>>wat_vec_dataidx|   $i:wat_dataidx   $is:wat_dataidx  * <<) =>
+    `(Vec.cons >>wat_dataidx| $i<<   >>wat_vec_dataidx| $is*   << sorry)
+| `(>>wat_vec_localidx|  $i:wat_localidx  $is:wat_localidx * <<) =>
+    `(Vec.cons >>wat_localidx| $i<<  >>wat_vec_localidx| $is*  << sorry )
+| `(>>wat_vec_labelidx|  $i:wat_labelidx  $is:wat_labelidx * <<) =>
+    `(Vec.cons >>wat_labelidx| $i<<  >>wat_vec_labelidx| $is*  << sorry )
+
+| `(>>wat_vec_typeidx|   <<) => `(Vec.nil)
+| `(>>wat_vec_funcidx|   <<) => `(Vec.nil)
+| `(>>wat_vec_tableidx|  <<) => `(Vec.nil)
+| `(>>wat_vec_memidx|    <<) => `(Vec.nil)
+| `(>>wat_vec_globalidx| <<) => `(Vec.nil)
+| `(>>wat_vec_elemidx|   <<) => `(Vec.nil)
+| `(>>wat_vec_dataidx|   <<) => `(Vec.nil)
+| `(>>wat_vec_localidx|  <<) => `(Vec.nil)
+| `(>>wat_vec_labelidx|  <<) => `(Vec.nil)
 
 declare_syntax_cat wat_typeuse
 scoped syntax "(" "type" wat_typeidx ")" : wat_typeuse
 scoped syntax "(" "type" wat_typeidx ")" wat_param* wat_result* : wat_typeuse
 scoped syntax wat_param* wat_result* : wat_typeuse
 
-scoped syntax "[wat_typeuse|" wat_typeuse "]" : term
+scoped syntax ">>wat_typeuse|" wat_typeuse "<<" : term
 
 macro_rules
-| `([wat_typeuse| (type $x)]) => `(Typeuse.type_ind [wat_typeidx| $x])
-| `([wat_typeuse| (type $x) $t₁:wat_param* $t₂:wat_result*]) =>
-    `(Typeuse.param_res [wat_typeidx| $x]
-      [wat_param_list| $t₁*]
-      [wat_result_list| $t₂*]
+| `(>>wat_typeuse| (type $x)<<) => `(Typeuse.type_ind >>wat_typeidx| $x<<)
+| `(>>wat_typeuse| (type $x) $t₁:wat_param* $t₂:wat_result*<<) =>
+    `(Typeuse.param_res >>wat_typeidx| $x<<
+      >>wat_param_list| $t₁*<<
+      >>wat_result_list| $t₂*<<
     )
-| `([wat_typeuse| $t₁:wat_param* $t₂:wat_result*]) =>
-    `(Typeuse.elab_param_res [wat_param_list| $t₁*] [wat_result_list| $t₂*])
+| `(>>wat_typeuse| $t₁:wat_param* $t₂:wat_result*<<) =>
+    `(Typeuse.elab_param_res >>wat_param_list| $t₁*<< >>wat_result_list| $t₂*<<)
