Wasm/Text/Notation/Instr.lean
@@ -12,12 +12,12 @@ declare_syntax_cat wat_label
 scoped syntax wat_ident ?  : wat_label
 scoped syntax "↑" term:max : wat_label
 
-scoped syntax "[wat_label|" wat_label "]" : term
+scoped syntax ">>wat_label|" wat_label "<<" : term
 
 macro_rules
-| `([wat_label| $v:wat_ident ]) => `(Label.name [wat_ident| $v])
-| `([wat_label| ])              => `(Label.no_label)
-| `([wat_label| ↑$e])           => `($e)
+| `(>>wat_label| $v:wat_ident <<) => `(Label.name >>wat_ident| $v<<)
+| `(>>wat_label| <<)              => `(Label.no_label)
+| `(>>wat_label| ↑$e<<)           => `($e)
 
 /- Memory Args -/
 declare_syntax_cat wat_offset
@@ -33,70 +33,70 @@ scoped syntax wat_offset ? wat_align ? : wat_memarg₂
 scoped syntax wat_offset ? wat_align ? : wat_memarg₄
 scoped syntax wat_offset ? wat_align ? : wat_memarg₈
 
-scoped syntax "[wat_offset|" wat_offset ? "]" : term
-scoped syntax "[wat_align₁|" wat_align ? "]"   : term
-scoped syntax "[wat_align₂|" wat_align ? "]"   : term
-scoped syntax "[wat_align₄|" wat_align ? "]"   : term
-scoped syntax "[wat_align₈|" wat_align ? "]"   : term
-scoped syntax "[wat_memarg₁|" wat_memarg₁ "]" : term
-scoped syntax "[wat_memarg₂|" wat_memarg₂ "]" : term
-scoped syntax "[wat_memarg₄|" wat_memarg₄ "]" : term
-scoped syntax "[wat_memarg₈|" wat_memarg₈ "]" : term
+scoped syntax ">>wat_offset|" wat_offset ? "<<" : term
+scoped syntax ">>wat_align₁|" wat_align ? "<<"   : term
+scoped syntax ">>wat_align₂|" wat_align ? "<<"   : term
+scoped syntax ">>wat_align₄|" wat_align ? "<<"   : term
+scoped syntax ">>wat_align₈|" wat_align ? "<<"   : term
+scoped syntax ">>wat_memarg₁|" wat_memarg₁ "<<" : term
+scoped syntax ">>wat_memarg₂|" wat_memarg₂ "<<" : term
+scoped syntax ">>wat_memarg₄|" wat_memarg₄ "<<" : term
+scoped syntax ">>wat_memarg₈|" wat_memarg₈ "<<" : term
 
 macro_rules
-| `([wat_offset| ]) => `([wat_u32| 0])
-| `([wat_offset| offset=$o:wat_u32]) => `([wat_u32| $o])
+| `(>>wat_offset| <<) => `(>>wat_u32| 0<<)
+| `(>>wat_offset| offset=$o:wat_u32<<) => `(>>wat_u32| $o<<)
 
 macro_rules
-| `([wat_align₁| align=$a:wat_u32]) =>
-    `(Unsigned.ofNat (n:=⟨32, by simp⟩) (Nat.log 2 [wat_u32| $a].toNat))
-| `([wat_align₁| ]) => `([wat_u32| 0])
-| `([wat_align₂| align=$a:wat_u32]) =>
-    `(Unsigned.ofNat (n:=⟨32, by simp⟩) (Nat.log 2 [wat_u32| $a].toNat))
-| `([wat_align₂| ]) => `([wat_u32| 1])
-| `([wat_align₄| align=$a:wat_u32]) =>
-    `(Unsigned.ofNat (n:=⟨32, by simp⟩) (Nat.log 2 [wat_u32| $a].toNat))
-| `([wat_align₄| ]) => `([wat_u32| 2])
-| `([wat_align₈| align=$a:wat_u32]) =>
-    `(Unsigned.ofNat (n:=⟨32, by simp⟩) (Nat.log 2 [wat_u32| $a].toNat))
-| `([wat_align₈| ]) => `([wat_u32| 3])
+| `(>>wat_align₁| align=$a:wat_u32<<) =>
+    `(Unsigned.ofNat (n:=⟨32, by simp⟩) (Nat.log 2 >>wat_u32| $a<<.toNat))
+| `(>>wat_align₁| <<) => `(>>wat_u32| 0<<)
+| `(>>wat_align₂| align=$a:wat_u32<<) =>
+    `(Unsigned.ofNat (n:=⟨32, by simp⟩) (Nat.log 2 >>wat_u32| $a<<.toNat))
+| `(>>wat_align₂| <<) => `(>>wat_u32| 1<<)
+| `(>>wat_align₄| align=$a:wat_u32<<) =>
+    `(Unsigned.ofNat (n:=⟨32, by simp⟩) (Nat.log 2 >>wat_u32| $a<<.toNat))
+| `(>>wat_align₄| <<) => `(>>wat_u32| 2<<)
+| `(>>wat_align₈| align=$a:wat_u32<<) =>
+    `(Unsigned.ofNat (n:=⟨32, by simp⟩) (Nat.log 2 >>wat_u32| $a<<.toNat))
+| `(>>wat_align₈| <<) => `(>>wat_u32| 3<<)
 
 macro_rules
-| `([wat_memarg₁| $o:wat_offset $a:wat_align ]) =>
-    `(Syntax.Instr.Memory.Arg.mk [wat_offset| $o] [wat_align₁| $a])
-| `([wat_memarg₁| $o:wat_offset ]) =>
-    `(Syntax.Instr.Memory.Arg.mk [wat_offset| $o] [wat_align₁| ])
-| `([wat_memarg₁| $a:wat_align ]) =>
-    `(Syntax.Instr.Memory.Arg.mk [wat_offset| ] [wat_align₁| $a])
-| `([wat_memarg₁| ]) =>
-    `(Syntax.Instr.Memory.Arg.mk [wat_offset| ] [wat_align₁| ])
+| `(>>wat_memarg₁| $o:wat_offset $a:wat_align <<) =>
+    `(Syntax.Instr.Memory.Arg.mk >>wat_offset| $o<< >>wat_align₁| $a<<)
+| `(>>wat_memarg₁| $o:wat_offset <<) =>
+    `(Syntax.Instr.Memory.Arg.mk >>wat_offset| $o<< >>wat_align₁| <<)
+| `(>>wat_memarg₁| $a:wat_align <<) =>
+    `(Syntax.Instr.Memory.Arg.mk >>wat_offset| << >>wat_align₁| $a<<)
+| `(>>wat_memarg₁| <<) =>
+    `(Syntax.Instr.Memory.Arg.mk >>wat_offset| << >>wat_align₁| <<)
 
-| `([wat_memarg₂| $o:wat_offset $a:wat_align ]) =>
-    `(Syntax.Instr.Memory.Arg.mk [wat_offset| $o] [wat_align₂| $a])
-| `([wat_memarg₂| $o:wat_offset ]) =>
-    `(Syntax.Instr.Memory.Arg.mk [wat_offset| $o] [wat_align₂| ])
-| `([wat_memarg₂| $a:wat_align ]) =>
-    `(Syntax.Instr.Memory.Arg.mk [wat_offset| ] [wat_align₂| $a])
-| `([wat_memarg₂| ]) =>
-    `(Syntax.Instr.Memory.Arg.mk [wat_offset| ] [wat_align₂| ])
+| `(>>wat_memarg₂| $o:wat_offset $a:wat_align <<) =>
+    `(Syntax.Instr.Memory.Arg.mk >>wat_offset| $o<< >>wat_align₂| $a<<)
+| `(>>wat_memarg₂| $o:wat_offset <<) =>
+    `(Syntax.Instr.Memory.Arg.mk >>wat_offset| $o<< >>wat_align₂| <<)
+| `(>>wat_memarg₂| $a:wat_align <<) =>
+    `(Syntax.Instr.Memory.Arg.mk >>wat_offset| << >>wat_align₂| $a<<)
+| `(>>wat_memarg₂| <<) =>
+    `(Syntax.Instr.Memory.Arg.mk >>wat_offset| << >>wat_align₂| <<)
 
-| `([wat_memarg₄| $o:wat_offset $a:wat_align ]) =>
-    `(Syntax.Instr.Memory.Arg.mk [wat_offset| $o] [wat_align₄| $a])
-| `([wat_memarg₄| $o:wat_offset ]) =>
-    `(Syntax.Instr.Memory.Arg.mk [wat_offset| $o] [wat_align₄| ])
-| `([wat_memarg₄| $a:wat_align ]) =>
-    `(Syntax.Instr.Memory.Arg.mk [wat_offset| ] [wat_align₄| $a])
-| `([wat_memarg₄| ]) =>
-    `(Syntax.Instr.Memory.Arg.mk [wat_offset| ] [wat_align₄| ])
+| `(>>wat_memarg₄| $o:wat_offset $a:wat_align <<) =>
+    `(Syntax.Instr.Memory.Arg.mk >>wat_offset| $o<< >>wat_align₄| $a<<)
+| `(>>wat_memarg₄| $o:wat_offset <<) =>
+    `(Syntax.Instr.Memory.Arg.mk >>wat_offset| $o<< >>wat_align₄| <<)
+| `(>>wat_memarg₄| $a:wat_align <<) =>
+    `(Syntax.Instr.Memory.Arg.mk >>wat_offset| << >>wat_align₄| $a<<)
+| `(>>wat_memarg₄| <<) =>
+    `(Syntax.Instr.Memory.Arg.mk >>wat_offset| << >>wat_align₄| <<)
 
-| `([wat_memarg₈| $o:wat_offset $a:wat_align ]) =>
-    `(Syntax.Instr.Memory.Arg.mk [wat_offset| $o] [wat_align₈| $a])
-| `([wat_memarg₈| $o:wat_offset ]) =>
-    `(Syntax.Instr.Memory.Arg.mk [wat_offset| $o] [wat_align₈| ])
-| `([wat_memarg₈| $a:wat_align ]) =>
-    `(Syntax.Instr.Memory.Arg.mk [wat_offset| ] [wat_align₈| $a])
-| `([wat_memarg₈| ]) =>
-    `(Syntax.Instr.Memory.Arg.mk [wat_offset| ] [wat_align₈| ])
+| `(>>wat_memarg₈| $o:wat_offset $a:wat_align <<) =>
+    `(Syntax.Instr.Memory.Arg.mk >>wat_offset| $o<< >>wat_align₈| $a<<)
+| `(>>wat_memarg₈| $o:wat_offset <<) =>
+    `(Syntax.Instr.Memory.Arg.mk >>wat_offset| $o<< >>wat_align₈| <<)
+| `(>>wat_memarg₈| $a:wat_align <<) =>
+    `(Syntax.Instr.Memory.Arg.mk >>wat_offset| << >>wat_align₈| $a<<)
+| `(>>wat_memarg₈| <<) =>
+    `(Syntax.Instr.Memory.Arg.mk >>wat_offset| << >>wat_align₈| <<)
 
 
 /- Plain Instructions -/
@@ -316,144 +316,144 @@ scoped syntax "i64.extend32_s" : wat_plaininstr
 
 -- todo vector instruction :)
 
-scoped syntax "[wat_plaininstr|" wat_plaininstr "]" : term
+scoped syntax ">>wat_plaininstr|" wat_plaininstr "<<" : term
 
 macro_rules
-| `([wat_plaininstr| unreachable]) => `(Plain.unreachable)
-| `([wat_plaininstr| nop])         => `(Plain.nop)
-| `([wat_plaininstr| br $l])       => `(Plain.br [wat_labelidx| $l])
-| `([wat_plaininstr| br_if $l])    => `(Plain.br_if [wat_labelidx| $l])
-| `([wat_plaininstr| br_table $l:wat_labelidx $ls:wat_labelidx*]) =>
-    `(let l' := [wat_labelidx| $l]
-      let vec := Vec.cons l' [wat_vec_labelidx| $l $ls*] sorry
+| `(>>wat_plaininstr| unreachable<<) => `(Plain.unreachable)
+| `(>>wat_plaininstr| nop<<)         => `(Plain.nop)
+| `(>>wat_plaininstr| br $l<<)       => `(Plain.br >>wat_labelidx| $l<<)
+| `(>>wat_plaininstr| br_if $l<<)    => `(Plain.br_if >>wat_labelidx| $l<<)
+| `(>>wat_plaininstr| br_table $l:wat_labelidx $ls:wat_labelidx*<<) =>
+    `(let l' := >>wat_labelidx| $l<<
+      let vec := Vec.cons l' >>wat_vec_labelidx| $l $ls*<< sorry
       Plain.br_table (vec.dropLast) (vec.getLastD l')
     )
-| `([wat_plaininstr| return])                   => `(Plain.wasm_return)
-| `([wat_plaininstr| call $x:wat_funcidx])      =>
-    `(Plain.call [wat_funcidx| $x])
-| `([wat_plaininstr| call_indirect $x:wat_tableidx $y:wat_typeuse]) =>
-    `(Plain.call_indirect [wat_tableidx| $x] [wat_typeuse| $y])
-| `([wat_plaininstr| call_indirect $y:wat_typeuse]) =>
-    `(Plain.call_indirect [wat_tableidx| 0] [wat_typeuse| $y])
+| `(>>wat_plaininstr| return<<)                   => `(Plain.wasm_return)
+| `(>>wat_plaininstr| call $x:wat_funcidx<<)      =>
+    `(Plain.call >>wat_funcidx| $x<<)
+| `(>>wat_plaininstr| call_indirect $x:wat_tableidx $y:wat_typeuse<<) =>
+    `(Plain.call_indirect >>wat_tableidx| $x<< >>wat_typeuse| $y<<)
+| `(>>wat_plaininstr| call_indirect $y:wat_typeuse<<) =>
+    `(Plain.call_indirect >>wat_tableidx| 0<< >>wat_typeuse| $y<<)
 
 -- Reference
 macro_rules
-| `([wat_plaininstr| ref.null $t:wat_heaptype]) =>
-    `(Plain.reference <| .null [wat_heaptype| $t])
-| `([wat_plaininstr| ref.is_null]) => `(Plain.reference <| .is_null)
-| `([wat_plaininstr| ref.func $x:wat_funcidx]) =>
-    `(Plain.reference <| .func [wat_funcidx| $x])
+| `(>>wat_plaininstr| ref.null $t:wat_heaptype<<) =>
+    `(Plain.reference <| .null >>wat_heaptype| $t<<)
+| `(>>wat_plaininstr| ref.is_null<<) => `(Plain.reference <| .is_null)
+| `(>>wat_plaininstr| ref.func $x:wat_funcidx<<) =>
+    `(Plain.reference <| .func >>wat_funcidx| $x<<)
 
 -- Parametric
 macro_rules
-| `([wat_plaininstr| drop]) => `(Plain.drop)
-| `([wat_plaininstr| select]) => `(Plain.select .none)
-| `([wat_plaininstr| select $t:wat_result*]) =>
-    `(Plain.select (.some [wat_result_list| $t* ]))
+| `(>>wat_plaininstr| drop<<) => `(Plain.drop)
+| `(>>wat_plaininstr| select<<) => `(Plain.select .none)
+| `(>>wat_plaininstr| select $t:wat_result*<<) =>
+    `(Plain.select (.some >>wat_result_list| $t* <<))
 
 -- Variadic
 macro_rules
-| `([wat_plaininstr| local.get $x:wat_localidx]) =>
-    `(Plain.locl <| .get [wat_localidx| $x])
-| `([wat_plaininstr| local.set $x:wat_localidx]) =>
-    `(Plain.locl <| .set [wat_localidx| $x])
-| `([wat_plaininstr| local.tee $x:wat_localidx]) =>
-    `(Plain.locl <| .tee [wat_localidx| $x])
-| `([wat_plaininstr| global.get $x:wat_globalidx]) =>
-    `(Plain.globl <| .get [wat_globalidx| $x])
-| `([wat_plaininstr| global.set $x:wat_globalidx]) =>
-    `(Plain.globl <| .set [wat_globalidx| $x])
+| `(>>wat_plaininstr| local.get $x:wat_localidx<<) =>
+    `(Plain.locl <| .get >>wat_localidx| $x<<)
+| `(>>wat_plaininstr| local.set $x:wat_localidx<<) =>
+    `(Plain.locl <| .set >>wat_localidx| $x<<)
+| `(>>wat_plaininstr| local.tee $x:wat_localidx<<) =>
+    `(Plain.locl <| .tee >>wat_localidx| $x<<)
+| `(>>wat_plaininstr| global.get $x:wat_globalidx<<) =>
+    `(Plain.globl <| .get >>wat_globalidx| $x<<)
+| `(>>wat_plaininstr| global.set $x:wat_globalidx<<) =>
+    `(Plain.globl <| .set >>wat_globalidx| $x<<)
 
 -- Tables
 macro_rules
-| `([wat_plaininstr| table.get $x:wat_tableidx]) =>
-    `(Plain.table <| .get [wat_tableidx| $x])
-| `([wat_plaininstr| table.set $x:wat_tableidx]) =>
-    `(Plain.table <| .set [wat_tableidx| $x])
-| `([wat_plaininstr| table.size $x:wat_tableidx]) =>
-    `(Plain.table <| .size [wat_tableidx| $x])
-| `([wat_plaininstr| table.grow $x:wat_tableidx]) =>
-    `(Plain.table <| .grow [wat_tableidx| $x])
-| `([wat_plaininstr| table.fill $x:wat_tableidx]) =>
-    `(Plain.table <| .fill [wat_tableidx| $x])
-| `([wat_plaininstr| table.copy $x:wat_tableidx $y:wat_tableidx]) =>
-    `(Plain.table <| .copy [wat_tableidx| $x] [wat_tableidx| $y])
-| `([wat_plaininstr| table.init $x:wat_tableidx $y:wat_elemidx]) =>
-    `(Plain.table <| .init [wat_tableidx| $x] [wat_elemidx| $y])
-| `([wat_plaininstr| elem.drop $x:wat_elemidx]) =>
-    `(Plain.elem_drop [wat_elemidx| $x])
+| `(>>wat_plaininstr| table.get $x:wat_tableidx<<) =>
+    `(Plain.table <| .get >>wat_tableidx| $x<<)
+| `(>>wat_plaininstr| table.set $x:wat_tableidx<<) =>
+    `(Plain.table <| .set >>wat_tableidx| $x<<)
+| `(>>wat_plaininstr| table.size $x:wat_tableidx<<) =>
+    `(Plain.table <| .size >>wat_tableidx| $x<<)
+| `(>>wat_plaininstr| table.grow $x:wat_tableidx<<) =>
+    `(Plain.table <| .grow >>wat_tableidx| $x<<)
+| `(>>wat_plaininstr| table.fill $x:wat_tableidx<<) =>
+    `(Plain.table <| .fill >>wat_tableidx| $x<<)
+| `(>>wat_plaininstr| table.copy $x:wat_tableidx $y:wat_tableidx<<) =>
+    `(Plain.table <| .copy >>wat_tableidx| $x<< >>wat_tableidx| $y<<)
+| `(>>wat_plaininstr| table.init $x:wat_tableidx $y:wat_elemidx<<) =>
+    `(Plain.table <| .init >>wat_tableidx| $x<< >>wat_elemidx| $y<<)
+| `(>>wat_plaininstr| elem.drop $x:wat_elemidx<<) =>
+    `(Plain.elem_drop >>wat_elemidx| $x<<)
 -- Table Abbreviations
-| `([wat_plaininstr| table.get])  => `(Plain.table <| .get 0)
-| `([wat_plaininstr| table.set])  => `(Plain.table <| .set 0)
-| `([wat_plaininstr| table.size]) => `(Plain.table <| .size 0)
-| `([wat_plaininstr| table.grow]) => `(Plain.table <| .grow 0)
-| `([wat_plaininstr| table.fill]) => `(Plain.table <| .fill 0)
-| `([wat_plaininstr| table.copy]) => `(Plain.table <| .copy 0 0)
-| `([wat_plaininstr| table.init $x:wat_elemidx]) =>
-    `(Plain.table <| .init 0 [wat_elemidx| $x])
+| `(>>wat_plaininstr| table.get<<)  => `(Plain.table <| .get 0)
+| `(>>wat_plaininstr| table.set<<)  => `(Plain.table <| .set 0)
+| `(>>wat_plaininstr| table.size<<) => `(Plain.table <| .size 0)
+| `(>>wat_plaininstr| table.grow<<) => `(Plain.table <| .grow 0)
+| `(>>wat_plaininstr| table.fill<<) => `(Plain.table <| .fill 0)
+| `(>>wat_plaininstr| table.copy<<) => `(Plain.table <| .copy 0 0)
+| `(>>wat_plaininstr| table.init $x:wat_elemidx<<) =>
+    `(Plain.table <| .init 0 >>wat_elemidx| $x<<)
 
 -- Memory
 macro_rules
-| `([wat_plaininstr| i32.load $m]) =>
-  `(Plain.memory <| .integer (nn:=.double) (.load [wat_memarg₄| $m]))
-| `([wat_plaininstr| i64.load $m]) =>
-  `(Plain.memory <| .integer (nn:=.quad) (.load [wat_memarg₈| $m]))
-| `([wat_plaininstr| f32.load $m]) =>
-  `(Plain.memory <| .float (nn:=.double) (.load [wat_memarg₄| $m]))
-| `([wat_plaininstr| f64.load $m]) =>
-  `(Plain.memory <| .float (nn:=.quad) (.load [wat_memarg₈| $m]))
-| `([wat_plaininstr| i32.load8_s $m]) =>
-  `(Plain.memory <| .integer (nn:=.double) (.load8 .s [wat_memarg₁| $m]))
-| `([wat_plaininstr| i32.load8_u $m]) =>
-  `(Plain.memory <| .integer (nn:=.double) (.load8 .u [wat_memarg₁| $m]))
-| `([wat_plaininstr| i32.load16_s $m]) =>
-  `(Plain.memory <| .integer (nn:=.double) (.load16 .s [wat_memarg₂| $m]))
-| `([wat_plaininstr| i32.load16_u $m]) =>
-  `(Plain.memory <| .integer (nn:=.double) (.load16 .u [wat_memarg₂| $m]))
-| `([wat_plaininstr| i64.load8_s $m]) =>
-  `(Plain.memory <| .integer (nn:=.quad) (.load8 .s [wat_memarg₁| $m]))
-| `([wat_plaininstr| i64.load8_u $m]) =>
-  `(Plain.memory <| .integer (nn:=.quad) (.load8 .u [wat_memarg₁| $m]))
-| `([wat_plaininstr| i64.load16_s $m]) =>
-  `(Plain.memory <| .integer (nn:=.quad) (.load16 .s [wat_memarg₂| $m]))
-| `([wat_plaininstr| i64.load16_u $m]) =>
-  `(Plain.memory <| .integer (nn:=.quad) (.load16 .u [wat_memarg₂| $m]))
-| `([wat_plaininstr| i64.load32_s $m]) =>
-  `(Plain.memory <| .integer (nn:=.quad) (.load32 .s [wat_memarg₄| $m]))
-| `([wat_plaininstr| i64.load32_u $m]) =>
-  `(Plain.memory <| .integer (nn:=.quad) (.load32 .u [wat_memarg₄| $m]))
-| `([wat_plaininstr| i32.store $m]) =>
-  `(Plain.memory <| .integer (nn:=.double) (.store [wat_memarg₄| $m]))
-| `([wat_plaininstr| i64.store $m]) =>
-  `(Plain.memory <| .integer (nn:=.quad) (.store [wat_memarg₈| $m]))
-| `([wat_plaininstr| f32.store $m]) =>
-  `(Plain.memory <| .float (nn:=.double) (.store [wat_memarg₄| $m]))
-| `([wat_plaininstr| f64.store $m]) =>
-  `(Plain.memory <| .float (nn:=.quad) (.store [wat_memarg₈| $m]))
-| `([wat_plaininstr| i32.store8 $m]) =>
-  `(Plain.memory <| .integer (nn:=.double) (.store8 [wat_memarg₁| $m]))
-| `([wat_plaininstr| i32.store16 $m]) =>
-  `(Plain.memory <| .integer (nn:=.double) (.store16 [wat_memarg₂| $m]))
-| `([wat_plaininstr| i64.store8 $m]) =>
-  `(Plain.memory <| .integer (nn:=.quad) (.store8 [wat_memarg₁| $m]))
-| `([wat_plaininstr| i64.store16 $m]) =>
-  `(Plain.memory <| .integer (nn:=.quad) (.store16 [wat_memarg₂| $m]))
-| `([wat_plaininstr| i64.store32 $m]) =>
-  `(Plain.memory <| .integer (nn:=.quad) (.store32 [wat_memarg₄| $m]))
-| `([wat_plaininstr| memory.size]) => `(Plain.memory <| .size)
-| `([wat_plaininstr| memory.grow]) => `(Plain.memory <| .grow)
-| `([wat_plaininstr| memory.fill]) => `(Plain.memory <| .fill)
-| `([wat_plaininstr| memory.copy]) => `(Plain.memory <| .copy)
-| `([wat_plaininstr| memory.init $x]) =>
-    `(Plain.memory <| .init [wat_dataidx| $x])
-| `([wat_plaininstr| data.drop $x]) =>
-    `(Plain.memory <| .data_drop [wat_dataidx| $x])
+| `(>>wat_plaininstr| i32.load $m<<) =>
+  `(Plain.memory <| .integer (nn:=.double) (.load >>wat_memarg₄| $m<<))
+| `(>>wat_plaininstr| i64.load $m<<) =>
+  `(Plain.memory <| .integer (nn:=.quad) (.load >>wat_memarg₈| $m<<))
+| `(>>wat_plaininstr| f32.load $m<<) =>
+  `(Plain.memory <| .float (nn:=.double) (.load >>wat_memarg₄| $m<<))
+| `(>>wat_plaininstr| f64.load $m<<) =>
+  `(Plain.memory <| .float (nn:=.quad) (.load >>wat_memarg₈| $m<<))
+| `(>>wat_plaininstr| i32.load8_s $m<<) =>
+  `(Plain.memory <| .integer (nn:=.double) (.load8 .s >>wat_memarg₁| $m<<))
+| `(>>wat_plaininstr| i32.load8_u $m<<) =>
+  `(Plain.memory <| .integer (nn:=.double) (.load8 .u >>wat_memarg₁| $m<<))
+| `(>>wat_plaininstr| i32.load16_s $m<<) =>
+  `(Plain.memory <| .integer (nn:=.double) (.load16 .s >>wat_memarg₂| $m<<))
+| `(>>wat_plaininstr| i32.load16_u $m<<) =>
+  `(Plain.memory <| .integer (nn:=.double) (.load16 .u >>wat_memarg₂| $m<<))
+| `(>>wat_plaininstr| i64.load8_s $m<<) =>
+  `(Plain.memory <| .integer (nn:=.quad) (.load8 .s >>wat_memarg₁| $m<<))
+| `(>>wat_plaininstr| i64.load8_u $m<<) =>
+  `(Plain.memory <| .integer (nn:=.quad) (.load8 .u >>wat_memarg₁| $m<<))
+| `(>>wat_plaininstr| i64.load16_s $m<<) =>
+  `(Plain.memory <| .integer (nn:=.quad) (.load16 .s >>wat_memarg₂| $m<<))
+| `(>>wat_plaininstr| i64.load16_u $m<<) =>
+  `(Plain.memory <| .integer (nn:=.quad) (.load16 .u >>wat_memarg₂| $m<<))
+| `(>>wat_plaininstr| i64.load32_s $m<<) =>
+  `(Plain.memory <| .integer (nn:=.quad) (.load32 .s >>wat_memarg₄| $m<<))
+| `(>>wat_plaininstr| i64.load32_u $m<<) =>
+  `(Plain.memory <| .integer (nn:=.quad) (.load32 .u >>wat_memarg₄| $m<<))
+| `(>>wat_plaininstr| i32.store $m<<) =>
+  `(Plain.memory <| .integer (nn:=.double) (.store >>wat_memarg₄| $m<<))
+| `(>>wat_plaininstr| i64.store $m<<) =>
+  `(Plain.memory <| .integer (nn:=.quad) (.store >>wat_memarg₈| $m<<))
+| `(>>wat_plaininstr| f32.store $m<<) =>
+  `(Plain.memory <| .float (nn:=.double) (.store >>wat_memarg₄| $m<<))
+| `(>>wat_plaininstr| f64.store $m<<) =>
+  `(Plain.memory <| .float (nn:=.quad) (.store >>wat_memarg₈| $m<<))
+| `(>>wat_plaininstr| i32.store8 $m<<) =>
+  `(Plain.memory <| .integer (nn:=.double) (.store8 >>wat_memarg₁| $m<<))
+| `(>>wat_plaininstr| i32.store16 $m<<) =>
+  `(Plain.memory <| .integer (nn:=.double) (.store16 >>wat_memarg₂| $m<<))
+| `(>>wat_plaininstr| i64.store8 $m<<) =>
+  `(Plain.memory <| .integer (nn:=.quad) (.store8 >>wat_memarg₁| $m<<))
+| `(>>wat_plaininstr| i64.store16 $m<<) =>
+  `(Plain.memory <| .integer (nn:=.quad) (.store16 >>wat_memarg₂| $m<<))
+| `(>>wat_plaininstr| i64.store32 $m<<) =>
+  `(Plain.memory <| .integer (nn:=.quad) (.store32 >>wat_memarg₄| $m<<))
+| `(>>wat_plaininstr| memory.size<<) => `(Plain.memory <| .size)
+| `(>>wat_plaininstr| memory.grow<<) => `(Plain.memory <| .grow)
+| `(>>wat_plaininstr| memory.fill<<) => `(Plain.memory <| .fill)
+| `(>>wat_plaininstr| memory.copy<<) => `(Plain.memory <| .copy)
+| `(>>wat_plaininstr| memory.init $x<<) =>
+    `(Plain.memory <| .init >>wat_dataidx| $x<<)
+| `(>>wat_plaininstr| data.drop $x<<) =>
+    `(Plain.memory <| .data_drop >>wat_dataidx| $x<<)
 
 macro_rules
-| `([wat_plaininstr| i32.const $n]) =>
-    `(Plain.numeric (nn:=.double) <| .integer (.const [wat_i32| $n]))
-| `([wat_plaininstr| i64.const $n]) =>
-    `(Plain.numeric (nn:=.quad) <| .integer (.const [wat_i64| $n]))
+| `(>>wat_plaininstr| i32.const $n<<) =>
+    `(Plain.numeric (nn:=.double) <| .integer (.const >>wat_i32| $n<<))
+| `(>>wat_plaininstr| i64.const $n<<) =>
+    `(Plain.numeric (nn:=.quad) <| .integer (.const >>wat_i64| $n<<))
 -- todo f32/f64 const
 
 -- some helpers to make the macro_rules shorter/more readable
@@ -492,177 +492,177 @@ macro_rules
 @[inline] private def float64 := float .quad
 
 macro_rules
-| `([wat_plaininstr| i32.clz])    => `(i32_unop .clz)
-| `([wat_plaininstr| i32.ctz])    => `(i32_unop .ctz)
-| `([wat_plaininstr| i32.popcnt]) => `(i32_unop .popcnt)
-| `([wat_plaininstr| i32.add])    => `(i32_binop .add)
-| `([wat_plaininstr| i32.sub])    => `(i32_binop .sub)
-| `([wat_plaininstr| i32.mul])    => `(i32_binop .mul)
-| `([wat_plaininstr| i32.div_s])  => `(i32_binop (.div .s))
-| `([wat_plaininstr| i32.div_u])  => `(i32_binop (.div .u))
-| `([wat_plaininstr| i32.rem_s])  => `(i32_binop (.rem .s))
-| `([wat_plaininstr| i32.rem_u])  => `(i32_binop (.rem .u))
-| `([wat_plaininstr| i32.and])    => `(i32_binop .and)
-| `([wat_plaininstr| i32.or])     => `(i32_binop .or)
-| `([wat_plaininstr| i32.xor])    => `(i32_binop .xor)
-| `([wat_plaininstr| i32.shl])    => `(i32_binop .shl)
-| `([wat_plaininstr| i32.shr_s])  => `(i32_binop (.shr .s))
-| `([wat_plaininstr| i32.shr_u])  => `(i32_binop (.shr .u))
-| `([wat_plaininstr| i32.rotl])   => `(i32_binop .rotl)
-| `([wat_plaininstr| i32.rotr])   => `(i32_binop .rotr)
+| `(>>wat_plaininstr| i32.clz<<)    => `(i32_unop .clz)
+| `(>>wat_plaininstr| i32.ctz<<)    => `(i32_unop .ctz)
+| `(>>wat_plaininstr| i32.popcnt<<) => `(i32_unop .popcnt)
+| `(>>wat_plaininstr| i32.add<<)    => `(i32_binop .add)
+| `(>>wat_plaininstr| i32.sub<<)    => `(i32_binop .sub)
+| `(>>wat_plaininstr| i32.mul<<)    => `(i32_binop .mul)
+| `(>>wat_plaininstr| i32.div_s<<)  => `(i32_binop (.div .s))
+| `(>>wat_plaininstr| i32.div_u<<)  => `(i32_binop (.div .u))
+| `(>>wat_plaininstr| i32.rem_s<<)  => `(i32_binop (.rem .s))
+| `(>>wat_plaininstr| i32.rem_u<<)  => `(i32_binop (.rem .u))
+| `(>>wat_plaininstr| i32.and<<)    => `(i32_binop .and)
+| `(>>wat_plaininstr| i32.or<<)     => `(i32_binop .or)
+| `(>>wat_plaininstr| i32.xor<<)    => `(i32_binop .xor)
+| `(>>wat_plaininstr| i32.shl<<)    => `(i32_binop .shl)
+| `(>>wat_plaininstr| i32.shr_s<<)  => `(i32_binop (.shr .s))
+| `(>>wat_plaininstr| i32.shr_u<<)  => `(i32_binop (.shr .u))
+| `(>>wat_plaininstr| i32.rotl<<)   => `(i32_binop .rotl)
+| `(>>wat_plaininstr| i32.rotr<<)   => `(i32_binop .rotr)
 
 macro_rules
-| `([wat_plaininstr| i64.clz])    => `(i64_unop .clz)
-| `([wat_plaininstr| i64.ctz])    => `(i64_unop .ctz)
-| `([wat_plaininstr| i64.popcnt]) => `(i64_unop .popcnt)
-| `([wat_plaininstr| i64.add])    => `(i64_binop .add)
-| `([wat_plaininstr| i64.sub])    => `(i64_binop .sub)
-| `([wat_plaininstr| i64.mul])    => `(i64_binop .mul)
-| `([wat_plaininstr| i64.div_s])  => `(i64_binop (.div .s))
-| `([wat_plaininstr| i64.div_u])  => `(i64_binop (.div .u))
-| `([wat_plaininstr| i64.rem_s])  => `(i64_binop (.rem .s))
-| `([wat_plaininstr| i64.rem_u])  => `(i64_binop (.rem .u))
-| `([wat_plaininstr| i64.and])    => `(i64_binop .and)
-| `([wat_plaininstr| i64.or])     => `(i64_binop .or)
-| `([wat_plaininstr| i64.xor])    => `(i64_binop .xor)
-| `([wat_plaininstr| i64.shl])    => `(i64_binop .shl)
-| `([wat_plaininstr| i64.shr_s])  => `(i64_binop (.shr .s))
-| `([wat_plaininstr| i64.shr_u])  => `(i64_binop (.shr .u))
-| `([wat_plaininstr| i64.rotl])   => `(i64_binop .rotl)
-| `([wat_plaininstr| i64.rotr])   => `(i64_binop .rotr)
+| `(>>wat_plaininstr| i64.clz<<)    => `(i64_unop .clz)
+| `(>>wat_plaininstr| i64.ctz<<)    => `(i64_unop .ctz)
+| `(>>wat_plaininstr| i64.popcnt<<) => `(i64_unop .popcnt)
+| `(>>wat_plaininstr| i64.add<<)    => `(i64_binop .add)
+| `(>>wat_plaininstr| i64.sub<<)    => `(i64_binop .sub)
+| `(>>wat_plaininstr| i64.mul<<)    => `(i64_binop .mul)
+| `(>>wat_plaininstr| i64.div_s<<)  => `(i64_binop (.div .s))
+| `(>>wat_plaininstr| i64.div_u<<)  => `(i64_binop (.div .u))
+| `(>>wat_plaininstr| i64.rem_s<<)  => `(i64_binop (.rem .s))
+| `(>>wat_plaininstr| i64.rem_u<<)  => `(i64_binop (.rem .u))
+| `(>>wat_plaininstr| i64.and<<)    => `(i64_binop .and)
+| `(>>wat_plaininstr| i64.or<<)     => `(i64_binop .or)
+| `(>>wat_plaininstr| i64.xor<<)    => `(i64_binop .xor)
+| `(>>wat_plaininstr| i64.shl<<)    => `(i64_binop .shl)
+| `(>>wat_plaininstr| i64.shr_s<<)  => `(i64_binop (.shr .s))
+| `(>>wat_plaininstr| i64.shr_u<<)  => `(i64_binop (.shr .u))
+| `(>>wat_plaininstr| i64.rotl<<)   => `(i64_binop .rotl)
+| `(>>wat_plaininstr| i64.rotr<<)   => `(i64_binop .rotr)
 
 macro_rules
-| `([wat_plaininstr| f32.abs])      => `(f32_unop .abs)
-| `([wat_plaininstr| f32.neg])      => `(f32_unop .neg)
-| `([wat_plaininstr| f32.ceil])     => `(f32_unop .ceil)
-| `([wat_plaininstr| f32.floor])    => `(f32_unop .floor)
-| `([wat_plaininstr| f32.trunc])    => `(f32_unop .trunc)
-| `([wat_plaininstr| f32.nearest])  => `(f32_unop .nearest)
-| `([wat_plaininstr| f32.sqrt])     => `(f32_unop .sqrt)
-| `([wat_plaininstr| f32.add])      => `(f32_binop .add)
-| `([wat_plaininstr| f32.sub])      => `(f32_binop .sub)
-| `([wat_plaininstr| f32.mul])      => `(f32_binop .mul)
-| `([wat_plaininstr| f32.div])      => `(f32_binop .div)
-| `([wat_plaininstr| f32.min])      => `(f32_binop .min)
-| `([wat_plaininstr| f32.max])      => `(f32_binop .max)
-| `([wat_plaininstr| f32.copysign]) => `(f32_binop .copysign)
+| `(>>wat_plaininstr| f32.abs<<)      => `(f32_unop .abs)
+| `(>>wat_plaininstr| f32.neg<<)      => `(f32_unop .neg)
+| `(>>wat_plaininstr| f32.ceil<<)     => `(f32_unop .ceil)
+| `(>>wat_plaininstr| f32.floor<<)    => `(f32_unop .floor)
+| `(>>wat_plaininstr| f32.trunc<<)    => `(f32_unop .trunc)
+| `(>>wat_plaininstr| f32.nearest<<)  => `(f32_unop .nearest)
+| `(>>wat_plaininstr| f32.sqrt<<)     => `(f32_unop .sqrt)
+| `(>>wat_plaininstr| f32.add<<)      => `(f32_binop .add)
+| `(>>wat_plaininstr| f32.sub<<)      => `(f32_binop .sub)
+| `(>>wat_plaininstr| f32.mul<<)      => `(f32_binop .mul)
+| `(>>wat_plaininstr| f32.div<<)      => `(f32_binop .div)
+| `(>>wat_plaininstr| f32.min<<)      => `(f32_binop .min)
+| `(>>wat_plaininstr| f32.max<<)      => `(f32_binop .max)
+| `(>>wat_plaininstr| f32.copysign<<) => `(f32_binop .copysign)
 
 macro_rules
-| `([wat_plaininstr| f64.abs])      => `(f64_unop .abs)
-| `([wat_plaininstr| f64.neg])      => `(f64_unop .neg)
-| `([wat_plaininstr| f64.ceil])     => `(f64_unop .ceil)
-| `([wat_plaininstr| f64.floor])    => `(f64_unop .floor)
-| `([wat_plaininstr| f64.trunc])    => `(f64_unop .trunc)
-| `([wat_plaininstr| f64.nearest])  => `(f64_unop .nearest)
-| `([wat_plaininstr| f64.sqrt])     => `(f64_unop .sqrt)
-| `([wat_plaininstr| f64.add])      => `(f64_binop .add)
-| `([wat_plaininstr| f64.sub])      => `(f64_binop .sub)
-| `([wat_plaininstr| f64.mul])      => `(f64_binop .mul)
-| `([wat_plaininstr| f64.div])      => `(f64_binop .div)
-| `([wat_plaininstr| f64.min])      => `(f64_binop .min)
-| `([wat_plaininstr| f64.max])      => `(f64_binop .max)
-| `([wat_plaininstr| f64.copysign]) => `(f64_binop .copysign)
+| `(>>wat_plaininstr| f64.abs<<)      => `(f64_unop .abs)
+| `(>>wat_plaininstr| f64.neg<<)      => `(f64_unop .neg)
+| `(>>wat_plaininstr| f64.ceil<<)     => `(f64_unop .ceil)
+| `(>>wat_plaininstr| f64.floor<<)    => `(f64_unop .floor)
+| `(>>wat_plaininstr| f64.trunc<<)    => `(f64_unop .trunc)
+| `(>>wat_plaininstr| f64.nearest<<)  => `(f64_unop .nearest)
+| `(>>wat_plaininstr| f64.sqrt<<)     => `(f64_unop .sqrt)
+| `(>>wat_plaininstr| f64.add<<)      => `(f64_binop .add)
+| `(>>wat_plaininstr| f64.sub<<)      => `(f64_binop .sub)
+| `(>>wat_plaininstr| f64.mul<<)      => `(f64_binop .mul)
+| `(>>wat_plaininstr| f64.div<<)      => `(f64_binop .div)
+| `(>>wat_plaininstr| f64.min<<)      => `(f64_binop .min)
+| `(>>wat_plaininstr| f64.max<<)      => `(f64_binop .max)
+| `(>>wat_plaininstr| f64.copysign<<) => `(f64_binop .copysign)
 
 macro_rules
-| `([wat_plaininstr| i32.eqz])  => `(i32_eqz)
-| `([wat_plaininstr| i32.eq])   => `(i32_rel .eq)
-| `([wat_plaininstr| i32.ne])   => `(i32_rel .ne)
-| `([wat_plaininstr| i32.lt_s]) => `(i32_rel (.lt .s))
-| `([wat_plaininstr| i32.lt_u]) => `(i32_rel (.lt .u))
-| `([wat_plaininstr| i32.gt_s]) => `(i32_rel (.gt .s))
-| `([wat_plaininstr| i32.gt_u]) => `(i32_rel (.gt .u))
-| `([wat_plaininstr| i32.le_s]) => `(i32_rel (.le .s))
-| `([wat_plaininstr| i32.le_u]) => `(i32_rel (.le .u))
-| `([wat_plaininstr| i32.ge_s]) => `(i32_rel (.ge .s))
-| `([wat_plaininstr| i32.ge_u]) => `(i32_rel (.ge .u))
+| `(>>wat_plaininstr| i32.eqz<<)  => `(i32_eqz)
+| `(>>wat_plaininstr| i32.eq<<)   => `(i32_rel .eq)
+| `(>>wat_plaininstr| i32.ne<<)   => `(i32_rel .ne)
+| `(>>wat_plaininstr| i32.lt_s<<) => `(i32_rel (.lt .s))
+| `(>>wat_plaininstr| i32.lt_u<<) => `(i32_rel (.lt .u))
+| `(>>wat_plaininstr| i32.gt_s<<) => `(i32_rel (.gt .s))
+| `(>>wat_plaininstr| i32.gt_u<<) => `(i32_rel (.gt .u))
+| `(>>wat_plaininstr| i32.le_s<<) => `(i32_rel (.le .s))
+| `(>>wat_plaininstr| i32.le_u<<) => `(i32_rel (.le .u))
+| `(>>wat_plaininstr| i32.ge_s<<) => `(i32_rel (.ge .s))
+| `(>>wat_plaininstr| i32.ge_u<<) => `(i32_rel (.ge .u))
 
 macro_rules
-| `([wat_plaininstr| i64.eqz])  => `(i64_eqz)
-| `([wat_plaininstr| i64.eq])   => `(i64_rel .eq)
-| `([wat_plaininstr| i64.ne])   => `(i64_rel .ne)
-| `([wat_plaininstr| i64.lt_s]) => `(i64_rel (.lt .s))
-| `([wat_plaininstr| i64.lt_u]) => `(i64_rel (.lt .u))
-| `([wat_plaininstr| i64.gt_s]) => `(i64_rel (.gt .s))
-| `([wat_plaininstr| i64.gt_u]) => `(i64_rel (.gt .u))
-| `([wat_plaininstr| i64.le_s]) => `(i64_rel (.le .s))
-| `([wat_plaininstr| i64.le_u]) => `(i64_rel (.le .u))
-| `([wat_plaininstr| i64.ge_s]) => `(i64_rel (.ge .s))
-| `([wat_plaininstr| i64.ge_u]) => `(i64_rel (.ge .u))
+| `(>>wat_plaininstr| i64.eqz<<)  => `(i64_eqz)
+| `(>>wat_plaininstr| i64.eq<<)   => `(i64_rel .eq)
+| `(>>wat_plaininstr| i64.ne<<)   => `(i64_rel .ne)
+| `(>>wat_plaininstr| i64.lt_s<<) => `(i64_rel (.lt .s))
+| `(>>wat_plaininstr| i64.lt_u<<) => `(i64_rel (.lt .u))
+| `(>>wat_plaininstr| i64.gt_s<<) => `(i64_rel (.gt .s))
+| `(>>wat_plaininstr| i64.gt_u<<) => `(i64_rel (.gt .u))
+| `(>>wat_plaininstr| i64.le_s<<) => `(i64_rel (.le .s))
+| `(>>wat_plaininstr| i64.le_u<<) => `(i64_rel (.le .u))
+| `(>>wat_plaininstr| i64.ge_s<<) => `(i64_rel (.ge .s))
+| `(>>wat_plaininstr| i64.ge_u<<) => `(i64_rel (.ge .u))
 
 macro_rules
-| `([wat_plaininstr| f32.eq]) => `(f32_rel .eq)
-| `([wat_plaininstr| f32.ne]) => `(f32_rel .ne)
-| `([wat_plaininstr| f32.lt]) => `(f32_rel .lt)
-| `([wat_plaininstr| f32.gt]) => `(f32_rel .gt)
-| `([wat_plaininstr| f32.le]) => `(f32_rel .le)
-| `([wat_plaininstr| f32.ge]) => `(f32_rel .ge)
+| `(>>wat_plaininstr| f32.eq<<) => `(f32_rel .eq)
+| `(>>wat_plaininstr| f32.ne<<) => `(f32_rel .ne)
+| `(>>wat_plaininstr| f32.lt<<) => `(f32_rel .lt)
+| `(>>wat_plaininstr| f32.gt<<) => `(f32_rel .gt)
+| `(>>wat_plaininstr| f32.le<<) => `(f32_rel .le)
+| `(>>wat_plaininstr| f32.ge<<) => `(f32_rel .ge)
 
 macro_rules
-| `([wat_plaininstr| f64.eq]) => `(f64_rel .eq)
-| `([wat_plaininstr| f64.ne]) => `(f64_rel .ne)
-| `([wat_plaininstr| f64.lt]) => `(f64_rel .lt)
-| `([wat_plaininstr| f64.gt]) => `(f64_rel .gt)
-| `([wat_plaininstr| f64.le]) => `(f64_rel .le)
-| `([wat_plaininstr| f64.ge]) => `(f64_rel .ge)
+| `(>>wat_plaininstr| f64.eq<<) => `(f64_rel .eq)
+| `(>>wat_plaininstr| f64.ne<<) => `(f64_rel .ne)
+| `(>>wat_plaininstr| f64.lt<<) => `(f64_rel .lt)
+| `(>>wat_plaininstr| f64.gt<<) => `(f64_rel .gt)
+| `(>>wat_plaininstr| f64.le<<) => `(f64_rel .le)
+| `(>>wat_plaininstr| f64.ge<<) => `(f64_rel .ge)
 
 macro_rules
-| `([wat_plaininstr| i32.wrap_i64])        => `(int32 (.wrap_i64))
-| `([wat_plaininstr| i32.trunc_f32_s])     => `(int32 (.trunc_f .double .s))
-| `([wat_plaininstr| i32.trunc_f32_u])     => `(int32 (.trunc_f .double .u))
-| `([wat_plaininstr| i32.trunc_f64_s])     => `(int32 (.trunc_f .quad .s))
-| `([wat_plaininstr| i32.trunc_f64_u])     => `(int32 (.trunc_f .quad .u))
-| `([wat_plaininstr| i32.trunc_sat_f32_s]) => `(int32 (.trunc_sat_f .double .s))
-| `([wat_plaininstr| i32.trunc_sat_f32_u]) => `(int32 (.trunc_sat_f .double .u))
-| `([wat_plaininstr| i32.trunc_sat_f64_s]) => `(int32 (.trunc_sat_f .quad .s))
-| `([wat_plaininstr| i32.trunc_sat_f64_u]) => `(int32 (.trunc_sat_f .quad .u))
+| `(>>wat_plaininstr| i32.wrap_i64<<)        => `(int32 (.wrap_i64))
+| `(>>wat_plaininstr| i32.trunc_f32_s<<)     => `(int32 (.trunc_f .double .s))
+| `(>>wat_plaininstr| i32.trunc_f32_u<<)     => `(int32 (.trunc_f .double .u))
+| `(>>wat_plaininstr| i32.trunc_f64_s<<)     => `(int32 (.trunc_f .quad .s))
+| `(>>wat_plaininstr| i32.trunc_f64_u<<)     => `(int32 (.trunc_f .quad .u))
+| `(>>wat_plaininstr| i32.trunc_sat_f32_s<<) => `(int32 (.trunc_sat_f .double .s))
+| `(>>wat_plaininstr| i32.trunc_sat_f32_u<<) => `(int32 (.trunc_sat_f .double .u))
+| `(>>wat_plaininstr| i32.trunc_sat_f64_s<<) => `(int32 (.trunc_sat_f .quad .s))
+| `(>>wat_plaininstr| i32.trunc_sat_f64_u<<) => `(int32 (.trunc_sat_f .quad .u))
 
-| `([wat_plaininstr| i64.extend_i32_s])    => `(int64 (.extend_i32 .s))
-| `([wat_plaininstr| i64.extend_i32_u])    => `(int64 (.extend_i32 .u))
-| `([wat_plaininstr| i64.trunc_f32_s])     => `(int64 (.trunc_f .double .s))
-| `([wat_plaininstr| i64.trunc_f32_u])     => `(int64 (.trunc_f .double .u))
-| `([wat_plaininstr| i64.trunc_f64_s])     => `(int64 (.trunc_f .quad .s))
-| `([wat_plaininstr| i64.trunc_f64_u])     => `(int64 (.trunc_f .quad .u))
-| `([wat_plaininstr| i64.trunc_sat_f32_s]) => `(int64 (.trunc_sat_f .double .s))
-| `([wat_plaininstr| i64.trunc_sat_f32_u]) => `(int64 (.trunc_sat_f .double .u))
-| `([wat_plaininstr| i64.trunc_sat_f64_s]) => `(int64 (.trunc_sat_f .quad .s))
-| `([wat_plaininstr| i64.trunc_sat_f64_u]) => `(int64 (.trunc_sat_f .quad .u))
+| `(>>wat_plaininstr| i64.extend_i32_s<<)    => `(int64 (.extend_i32 .s))
+| `(>>wat_plaininstr| i64.extend_i32_u<<)    => `(int64 (.extend_i32 .u))
+| `(>>wat_plaininstr| i64.trunc_f32_s<<)     => `(int64 (.trunc_f .double .s))
+| `(>>wat_plaininstr| i64.trunc_f32_u<<)     => `(int64 (.trunc_f .double .u))
+| `(>>wat_plaininstr| i64.trunc_f64_s<<)     => `(int64 (.trunc_f .quad .s))
+| `(>>wat_plaininstr| i64.trunc_f64_u<<)     => `(int64 (.trunc_f .quad .u))
+| `(>>wat_plaininstr| i64.trunc_sat_f32_s<<) => `(int64 (.trunc_sat_f .double .s))
+| `(>>wat_plaininstr| i64.trunc_sat_f32_u<<) => `(int64 (.trunc_sat_f .double .u))
+| `(>>wat_plaininstr| i64.trunc_sat_f64_s<<) => `(int64 (.trunc_sat_f .quad .s))
+| `(>>wat_plaininstr| i64.trunc_sat_f64_u<<) => `(int64 (.trunc_sat_f .quad .u))
 
-| `([wat_plaininstr| f32.convert_i32_s]) => `(float32 (.convert_i .double .s))
-| `([wat_plaininstr| f32.convert_i32_u]) => `(float32 (.convert_i .double .u))
-| `([wat_plaininstr| f32.convert_i64_s]) => `(float32 (.convert_i .quad .s))
-| `([wat_plaininstr| f32.convert_i64_u]) => `(float32 (.convert_i .quad .u))
-| `([wat_plaininstr| f32.demote_f64])    => `(float32 (.demote_f64))
+| `(>>wat_plaininstr| f32.convert_i32_s<<) => `(float32 (.convert_i .double .s))
+| `(>>wat_plaininstr| f32.convert_i32_u<<) => `(float32 (.convert_i .double .u))
+| `(>>wat_plaininstr| f32.convert_i64_s<<) => `(float32 (.convert_i .quad .s))
+| `(>>wat_plaininstr| f32.convert_i64_u<<) => `(float32 (.convert_i .quad .u))
+| `(>>wat_plaininstr| f32.demote_f64<<)    => `(float32 (.demote_f64))
 
-| `([wat_plaininstr| f64.convert_i32_s]) => `(float64 (.convert_i .double .s))
-| `([wat_plaininstr| f64.convert_i32_u]) => `(float64 (.convert_i .double .u))
-| `([wat_plaininstr| f64.convert_i64_s]) => `(float64 (.convert_i .quad .s))
-| `([wat_plaininstr| f64.convert_i64_u]) => `(float64 (.convert_i .quad .u))
-| `([wat_plaininstr| f64.promote_f32])   => `(float64 (.promote_f32))
+| `(>>wat_plaininstr| f64.convert_i32_s<<) => `(float64 (.convert_i .double .s))
+| `(>>wat_plaininstr| f64.convert_i32_u<<) => `(float64 (.convert_i .double .u))
+| `(>>wat_plaininstr| f64.convert_i64_s<<) => `(float64 (.convert_i .quad .s))
+| `(>>wat_plaininstr| f64.convert_i64_u<<) => `(float64 (.convert_i .quad .u))
+| `(>>wat_plaininstr| f64.promote_f32<<)   => `(float64 (.promote_f32))
 
-| `([wat_plaininstr| i32.reinterpret_f32]) => `(int32 (.reinterpret_f))
-| `([wat_plaininstr| i64.reinterpret_f64]) => `(int64 (.reinterpret_f))
-| `([wat_plaininstr| f32.reinterpret_i32]) => `(float32 (.reinterpret_i))
-| `([wat_plaininstr| f64.reinterpret_i64]) => `(float64 (.reinterpret_i))
+| `(>>wat_plaininstr| i32.reinterpret_f32<<) => `(int32 (.reinterpret_f))
+| `(>>wat_plaininstr| i64.reinterpret_f64<<) => `(int64 (.reinterpret_f))
+| `(>>wat_plaininstr| f32.reinterpret_i32<<) => `(float32 (.reinterpret_i))
+| `(>>wat_plaininstr| f64.reinterpret_i64<<) => `(float64 (.reinterpret_i))
 
 macro_rules
-| `([wat_plaininstr| i32.extend8_s])  => `(int32 (.extend8_s))
-| `([wat_plaininstr| i32.extend16_s]) => `(int32 (.extend16_s))
-| `([wat_plaininstr| i64.extend8_s])  => `(int64 (.extend8_s))
-| `([wat_plaininstr| i64.extend16_s]) => `(int64 (.extend16_s))
-| `([wat_plaininstr| i64.extend32_s]) => `(int64 (.extend32_s))
+| `(>>wat_plaininstr| i32.extend8_s<<)  => `(int32 (.extend8_s))
+| `(>>wat_plaininstr| i32.extend16_s<<) => `(int32 (.extend16_s))
+| `(>>wat_plaininstr| i64.extend8_s<<)  => `(int64 (.extend8_s))
+| `(>>wat_plaininstr| i64.extend16_s<<) => `(int64 (.extend16_s))
+| `(>>wat_plaininstr| i64.extend32_s<<) => `(int64 (.extend32_s))
 
 declare_syntax_cat wat_blocktype
 scoped syntax wat_result ? : wat_blocktype
 scoped syntax wat_typeuse  : wat_blocktype
 
-scoped syntax "[wat_blocktype|" wat_blocktype "]" : term
+scoped syntax ">>wat_blocktype|" wat_blocktype "<<" : term
 
 macro_rules
-| `([wat_blocktype| ]) => `(Instr.BlockType.value .none)
-| `([wat_blocktype| $t:wat_result]) =>
-    `(Instr.BlockType.value (.some [wat_result| $t]))
-| `([wat_blocktype| $x:wat_typeuse]) =>
-    `(Instr.BlockType.typeuse [wat_typeuse| $x])
+| `(>>wat_blocktype| <<) => `(Instr.BlockType.value .none)
+| `(>>wat_blocktype| $t:wat_result<<) =>
+    `(Instr.BlockType.value (.some >>wat_result| $t<<))
+| `(>>wat_blocktype| $x:wat_typeuse<<) =>
+    `(Instr.BlockType.typeuse >>wat_typeuse| $x<<)
 
 declare_syntax_cat wat_blockinstr
 declare_syntax_cat wat_instr
@@ -677,46 +677,46 @@ scoped syntax "loop" wat_label wat_blocktype (wat_instr)* "end" wat_ident? : wat
 scoped syntax "if" wat_label wat_blocktype (wat_instr)* "else" wat_ident? (wat_instr)* "end" wat_ident? : wat_blockinstr
 scoped syntax "if" wat_label wat_blocktype (wat_instr)* "end" wat_ident? : wat_blockinstr
 
-scoped syntax "[wat_blockinstr|" wat_blockinstr "]" : term
-scoped syntax "[wat_instr|" wat_instr "]"           : term
-scoped syntax "[wat_instr_list|" wat_instr* "]"     : term
+scoped syntax ">>wat_blockinstr|" wat_blockinstr "<<" : term
+scoped syntax ">>wat_instr|" wat_instr "<<"           : term
+scoped syntax ">>wat_instr_list|" wat_instr* "<<"     : term
 
 macro_rules
-| `([wat_instr| $i:wat_plaininstr]) => `(Instr.plain [wat_plaininstr| $i])
-| `([wat_instr| $i:wat_blockinstr]) => `(Instr.block [wat_blockinstr| $i])
-| `([wat_instr| ($i:wat_instr)])    => `([wat_instr| $i])
-| `([wat_instr| ↑$e])               => `($e)
+| `(>>wat_instr| $i:wat_plaininstr<<) => `(Instr.plain >>wat_plaininstr| $i<<)
+| `(>>wat_instr| $i:wat_blockinstr<<) => `(Instr.block >>wat_blockinstr| $i<<)
+| `(>>wat_instr| ($i:wat_instr)<<)    => `(>>wat_instr| $i<<)
+| `(>>wat_instr| ↑$e<<)               => `($e)
 
 macro_rules
-| `([wat_instr_list| ]) => `([])
-| `([wat_instr_list| $i:wat_instr $is:wat_instr*]) =>
-    `([wat_instr| $i] :: [wat_instr_list| $is*])
+| `(>>wat_instr_list| <<) => `([])
+| `(>>wat_instr_list| $i:wat_instr $is:wat_instr*<<) =>
+    `(>>wat_instr| $i<< :: >>wat_instr_list| $is*<<)
 
 macro_rules
-| `([wat_blockinstr| block $l:wat_label $bt:wat_blocktype
-                        $is:wat_instr* end $id]) =>
-    `(Block.block [wat_label| $l] [wat_blocktype| $bt]
-        [wat_instr_list| $is*] .wasm_end [wat_ident?| $id])
+| `(>>wat_blockinstr| block $l:wat_label $bt:wat_blocktype
+                        $is:wat_instr* end $id<<) =>
+    `(Block.block >>wat_label| $l<< >>wat_blocktype| $bt<<
+        >>wat_instr_list| $is*<< .wasm_end >>wat_ident?| $id<<)
 -- Loop
-| `([wat_blockinstr| loop $l:wat_label $bt:wat_blocktype
-                        $is:wat_instr* end $id]) =>
-    `(Block.loop [wat_label| $l] [wat_blocktype| $bt]
-        [wat_instr_list| $is*] .wasm_end [wat_ident?| $id])
+| `(>>wat_blockinstr| loop $l:wat_label $bt:wat_blocktype
+                        $is:wat_instr* end $id<<) =>
+    `(Block.loop >>wat_label| $l<< >>wat_blocktype| $bt<<
+        >>wat_instr_list| $is*<< .wasm_end >>wat_ident?| $id<<)
 -- If
-| `([wat_blockinstr| if $l:wat_label $bt:wat_blocktype $is₁:wat_instr*
+| `(>>wat_blockinstr| if $l:wat_label $bt:wat_blocktype $is₁:wat_instr*
                      else $id₁:wat_ident? $is₂:wat_instr*
-                     end $id₂:wat_ident?]) =>
-    `(Block.wasm_if [wat_label| $l] [wat_blocktype| $bt]
-        [wat_instr_list| $is₁*]
-        .wasm_else [wat_ident?| $id₁] [wat_instr_list| $is₂*]
-        .wasm_end [wat_ident?| $id₂])
+                     end $id₂:wat_ident?<<) =>
+    `(Block.wasm_if >>wat_label| $l<< >>wat_blocktype| $bt<<
+        >>wat_instr_list| $is₁*<<
+        .wasm_else >>wat_ident?| $id₁<< >>wat_instr_list| $is₂*<<
+        .wasm_end >>wat_ident?| $id₂<<)
 
 -- Abbreviation for If
-| `([wat_blockinstr| if $l:wat_label $bt:wat_blocktype
-                        $is:wat_instr* end $id]) =>
-    `(Block.wasm_if [wat_label| $l] [wat_blocktype| $bt]
-        [wat_instr_list| $is*]
-        .wasm_else .none [] .wasm_end [wat_ident?| $id])
+| `(>>wat_blockinstr| if $l:wat_label $bt:wat_blocktype
+                        $is:wat_instr* end $id<<) =>
+    `(Block.wasm_if >>wat_label| $l<< >>wat_blocktype| $bt<<
+        >>wat_instr_list| $is*<<
+        .wasm_else .none [] .wasm_end >>wat_ident?| $id<<)
 
 -- Currently broken so commented out :)
 /-
@@ -731,39 +731,39 @@ scoped syntax "loop" wat_label wat_blocktype wat_instr* : wat_foldedinstr_at
 scoped syntax "if" wat_label wat_blocktype wat_foldedinstr "(" "then" wat_instr* ")"
           ("(" "else" wat_instr* ")")? : wat_foldedinstr_at
 
-scoped syntax "[wat_foldedinstr_at|" wat_foldedinstr_at "]" : term
-scoped syntax "[wat_foldedinstr|" wat_foldedinstr "]" : term
+scoped syntax ">>wat_foldedinstr_at|" wat_foldedinstr_at "<<" : term
+scoped syntax ">>wat_foldedinstr|" wat_foldedinstr "<<" : term
 
 macro_rules
-| `([wat_foldedinstr| ($i)]) => `([wat_foldedinstr_at| $i])
--- | `([wat_foldedinstr| ($i $is) ]) =>
-    -- `([wat_foldedinstr_at| $i] :: [wat_foldedinstr| $is])
+| `(>>wat_foldedinstr| ($i)<<) => `(>>wat_foldedinstr_at| $i<<)
+-- | `(>>wat_foldedinstr| ($i $is) <<) =>
+    -- `(>>wat_foldedinstr_at| $i<< :: >>wat_foldedinstr| $is<<)
 
 macro_rules
-| `([wat_foldedinstr_at| $i:wat_plaininstr $is:wat_foldedinstr]) =>
-    `([wat_foldedinstr| $is] ++ [wat_plaininstr| $i])
-| `([wat_foldedinstr| (block $l $bt $is:wat_instr*)]) =>
-    `([wat_instr| block $l $bt $is* end])
-| `([wat_foldedinstr| (loop $l $bt $is:wat_instr*)]) =>
-    `([wat_instr| loop $l $bt $is* end])
+| `(>>wat_foldedinstr_at| $i:wat_plaininstr $is:wat_foldedinstr<<) =>
+    `(>>wat_foldedinstr| $is<< ++ >>wat_plaininstr| $i<<)
+| `(>>wat_foldedinstr| (block $l $bt $is:wat_instr*)<<) =>
+    `(>>wat_instr| block $l $bt $is* end<<)
+| `(>>wat_foldedinstr| (loop $l $bt $is:wat_instr*)<<) =>
+    `(>>wat_instr| loop $l $bt $is* end<<)
 
 macro_rules
-| `([wat_foldedinstr_at| if $l $bt $cond (then $is₁*) ]) =>
-    `([wat_foldedinstr| $cond] ++ [[wat_instr| if $l $bt $is₁* end]])
-| `([wat_foldedinstr| (if $l $bt $cond (then $is₁*) (else $is₂*) )]) =>
-    `([wat_foldedinstr| $cond]
-    ++ [[wat_instr| if $l $bt $is₁* else $is₂:wat_instr* end]])
+| `(>>wat_foldedinstr_at| if $l $bt $cond (then $is₁*) <<) =>
+    `(>>wat_foldedinstr| $cond<< ++ [>>wat_instr| if $l $bt $is₁* end<<])
+| `(>>wat_foldedinstr| (if $l $bt $cond (then $is₁*) (else $is₂*) )<<) =>
+    `(>>wat_foldedinstr| $cond<<
+    ++ [>>wat_instr| if $l $bt $is₁* else $is₂:wat_instr* end<<])
 
 scoped syntax wat_foldedinstr : wat_instr
 scoped syntax "(" wat_instr ")" : wat_instr
 macro_rules
-| `([wat_instr| $i:wat_foldedinstr]) => `([wat_foldedinstr| $i])
-| `([wat_instr| ($i:wat_instr)]) => `([wat_instr| $i])
+| `(>>wat_instr| $i:wat_foldedinstr<<) => `(>>wat_foldedinstr| $i<<)
+| `(>>wat_instr| ($i:wat_instr)<<) => `(>>wat_instr| $i<<)
 -/
 
 declare_syntax_cat wat_expr
 scoped syntax wat_instr* : wat_expr
-scoped syntax "[wat_expr|" wat_expr "]" : term
+scoped syntax ">>wat_expr|" wat_expr "<<" : term
 
 macro_rules
-| `([wat_expr| $is:wat_instr*]) => `([wat_instr_list| $is*])
+| `(>>wat_expr| $is:wat_instr*<<) => `(>>wat_instr_list| $is*<<)
