Wasm/Text/Notation/Typ.lean
@@ -15,23 +15,23 @@ scoped syntax "i64" : wat_numtype
 scoped syntax "f32" : wat_numtype
 scoped syntax "f64" : wat_numtype
 
-scoped syntax "[wat_numtype|" wat_numtype "]" : term
+scoped syntax ">>wat_numtype|" wat_numtype "<<" : term
 
 macro_rules
-| `([wat_numtype| i32 ]) => `(Wasm.Syntax.Typ.Num.i32   )
-| `([wat_numtype| i64 ]) => `(Wasm.Syntax.Typ.Num.i64   )
-| `([wat_numtype| f32 ]) => `(Wasm.Syntax.Typ.Num.f32   )
-| `([wat_numtype| f64 ]) => `(Wasm.Syntax.Typ.Num.f64   )
+| `(>>wat_numtype| i32 <<) => `(Wasm.Syntax.Typ.Num.i32   )
+| `(>>wat_numtype| i64 <<) => `(Wasm.Syntax.Typ.Num.i64   )
+| `(>>wat_numtype| f32 <<) => `(Wasm.Syntax.Typ.Num.f32   )
+| `(>>wat_numtype| f64 <<) => `(Wasm.Syntax.Typ.Num.f64   )
 
 
 /- Vector Types -/
 declare_syntax_cat wat_vectype
 scoped syntax "v128" : wat_vectype
 
-scoped syntax "[wat_vectype|" wat_vectype "]" : term
+scoped syntax ">>wat_vectype|" wat_vectype "<<" : term
 
 macro_rules
-| `([wat_vectype| v128 ]) => `(Wasm.Syntax.Typ.Vec.v128)
+| `(>>wat_vectype| v128 <<) => `(Wasm.Syntax.Typ.Vec.v128)
 
 
 /- Reference Types -/
@@ -43,16 +43,16 @@ scoped syntax "externref" : wat_reftype
 scoped syntax "func"   : wat_heaptype
 scoped syntax "extern" : wat_heaptype
 
-scoped syntax "[wat_reftype|" wat_reftype "]"   : term
-scoped syntax "[wat_heaptype|" wat_heaptype "]" : term
+scoped syntax ">>wat_reftype|" wat_reftype "<<"   : term
+scoped syntax ">>wat_heaptype|" wat_heaptype "<<" : term
 
 macro_rules
-| `([wat_reftype| funcref   ]) => `(Wasm.Syntax.Typ.Ref.func  )
-| `([wat_reftype| externref ]) => `(Wasm.Syntax.Typ.Ref.extern)
+| `(>>wat_reftype| funcref   <<) => `(Wasm.Syntax.Typ.Ref.func  )
+| `(>>wat_reftype| externref <<) => `(Wasm.Syntax.Typ.Ref.extern)
 
 macro_rules
-| `([wat_heaptype| func   ]) => `(Wasm.Syntax.Typ.Ref.func  )
-| `([wat_heaptype| extern ]) => `(Wasm.Syntax.Typ.Ref.extern)
+| `(>>wat_heaptype| func   <<) => `(Wasm.Syntax.Typ.Ref.func  )
+| `(>>wat_heaptype| extern <<) => `(Wasm.Syntax.Typ.Ref.extern)
 
 
 /- Value Types -/
@@ -61,12 +61,12 @@ scoped syntax wat_numtype : wat_valtype
 scoped syntax wat_vectype : wat_valtype
 scoped syntax wat_reftype : wat_valtype
 
-scoped syntax "[wat_valtype|" wat_valtype "]" : term
+scoped syntax ">>wat_valtype|" wat_valtype "<<" : term
 
 macro_rules
-| `([wat_valtype| $t:wat_numtype]) => `(Val.num [wat_numtype| $t])
-| `([wat_valtype| $t:wat_vectype]) => `(Val.vec [wat_vectype| $t])
-| `([wat_valtype| $t:wat_reftype]) => `(Val.ref [wat_reftype| $t])
+| `(>>wat_valtype| $t:wat_numtype<<) => `(Val.num >>wat_numtype| $t<<)
+| `(>>wat_valtype| $t:wat_vectype<<) => `(Val.vec >>wat_vectype| $t<<)
+| `(>>wat_valtype| $t:wat_reftype<<) => `(Val.ref >>wat_reftype| $t<<)
 
 
 /- Parameters -/
@@ -78,30 +78,30 @@ scoped syntax "(" "param" (wat_ident)? wat_valtype ")" : wat_param_core
 scoped syntax "(" "param" wat_valtype* ")" : wat_param
 scoped syntax wat_param_core               : wat_param
 
-scoped syntax "[wat_param_core|" wat_param_core "]" : term
-scoped syntax "[wat_param|" wat_param "]"           : term
-scoped syntax "[wat_param_list|" wat_param* "]"     : term
+scoped syntax ">>wat_param_core|" wat_param_core "<<" : term
+scoped syntax ">>wat_param|" wat_param "<<"           : term
+scoped syntax ">>wat_param_list|" wat_param* "<<"     : term
 
 macro_rules
-| `([wat_param_core| (param $t:wat_valtype)]) =>
-    `(Typ.Param.mk .none [wat_valtype| $t])
-| `([wat_param_core| (param $id:wat_ident $t:wat_valtype)]) =>
-    `(Typ.Param.mk (.some [wat_ident| $id]) [wat_valtype| $t])
+| `(>>wat_param_core| (param $t:wat_valtype)<<) =>
+    `(Typ.Param.mk .none >>wat_valtype| $t<<)
+| `(>>wat_param_core| (param $id:wat_ident $t:wat_valtype)<<) =>
+    `(Typ.Param.mk (.some >>wat_ident| $id<<) >>wat_valtype| $t<<)
 
 macro_rules
-| `([wat_param| (param $t:wat_valtype $ts:wat_valtype)]) =>
-    `([wat_param_core| (param $t)] :: [wat_param| (param $ts)])
-| `([wat_param| (param $t:wat_valtype )]) =>
-    `([[wat_param_core| (param $t)]])
-| `([wat_param| (param )]) => `([]) -- todo: double check this is valid
-| `([wat_param| $p:wat_param_core]) =>
-    `([wat_param_core| $p])
+| `(>>wat_param| (param $t:wat_valtype $ts:wat_valtype)<<) =>
+    `(>>wat_param_core| (param $t)<< :: >>wat_param| (param $ts)<<)
+| `(>>wat_param| (param $t:wat_valtype )<<) =>
+    `([>>wat_param_core| (param $t)<<])
+| `(>>wat_param| (param )<<) => `([]) -- todo: double check this is valid
+| `(>>wat_param| $p:wat_param_core<<) =>
+    `(>>wat_param_core| $p<<)
 
 macro_rules
-| `([wat_param_list| ]) => `([])
-| `([wat_param_list| $p:wat_param]) => `([[wat_param| $p]])
-| `([wat_param_list| $p:wat_param $ps:wat_param*]) =>
-    `([wat_param| $p] :: [wat_param_list| $ps*])
+| `(>>wat_param_list| <<) => `([])
+| `(>>wat_param_list| $p:wat_param<<) => `([>>wat_param| $p<<])
+| `(>>wat_param_list| $p:wat_param $ps:wat_param*<<) =>
+    `(>>wat_param| $p<< :: >>wat_param_list| $ps*<<)
 
 
 /- Results -/
@@ -112,36 +112,36 @@ scoped syntax "(" "result" wat_valtype ")"  : wat_result_core
 scoped syntax wat_result_core               : wat_result
 scoped syntax "(" "result" wat_valtype* ")" : wat_result
 
-scoped syntax "[wat_result_core|" wat_result_core "]" : term
-scoped syntax "[wat_result|" wat_result "]"           : term
-scoped syntax "[wat_result_list|" wat_result* "]"     : term
+scoped syntax ">>wat_result_core|" wat_result_core "<<" : term
+scoped syntax ">>wat_result|" wat_result "<<"           : term
+scoped syntax ">>wat_result_list|" wat_result* "<<"     : term
 
 macro_rules
-| `([wat_result_core| (result $t:wat_valtype)]) => `([wat_valtype| $t])
+| `(>>wat_result_core| (result $t:wat_valtype)<<) => `(>>wat_valtype| $t<<)
 
 macro_rules
-| `([wat_result| (result $r:wat_valtype $rs:wat_valtype)]) =>
-    `([wat_result_core| (result $r)] :: [wat_result| (result $rs)])
-| `([wat_result| (result $t:wat_valtype )]) =>
-    `([[wat_result_core| (result $t)]])
-| `([wat_result| (result )]) => `([]) -- todo: double check this is valid
-| `([wat_result| $r:wat_result_core]) =>
-    `([wat_result_core| $r])
+| `(>>wat_result| (result $r:wat_valtype $rs:wat_valtype)<<) =>
+    `(>>wat_result_core| (result $r)<< :: >>wat_result| (result $rs)<<)
+| `(>>wat_result| (result $t:wat_valtype )<<) =>
+    `([>>wat_result_core| (result $t)<<])
+| `(>>wat_result| (result )<<) => `([]) -- todo: double check this is valid
+| `(>>wat_result| $r:wat_result_core<<) =>
+    `(>>wat_result_core| $r<<)
 
 macro_rules
-| `([wat_result_list| ]) => `([])
-| `([wat_result_list| $r:wat_result]) => `([[wat_result| $r]])
-| `([wat_result_list| $r:wat_result $rs:wat_result*]) =>
-    `([wat_result| $r] :: [wat_result_list| $rs*])
+| `(>>wat_result_list| <<) => `([])
+| `(>>wat_result_list| $r:wat_result<<) => `([>>wat_result| $r<<])
+| `(>>wat_result_list| $r:wat_result $rs:wat_result*<<) =>
+    `(>>wat_result| $r<< :: >>wat_result_list| $rs*<<)
 
 
 /- Functions -/
 declare_syntax_cat wat_functype
 scoped syntax "(" "func" wat_param* wat_result* ")" : wat_functype
-scoped syntax "[wat_functype|" wat_functype "]" : term
+scoped syntax ">>wat_functype|" wat_functype "<<" : term
 macro_rules
-| `([wat_functype| (func $t₁:wat_param* $t₂:wat_result*)]) =>
-    `(Typ.Func.mk [wat_param_list| $t₁*] [wat_result_list| $t₂*])
+| `(>>wat_functype| (func $t₁:wat_param* $t₂:wat_result*)<<) =>
+    `(Typ.Func.mk >>wat_param_list| $t₁*<< >>wat_result_list| $t₂*<<)
 
 
 /- Limits -/
@@ -149,43 +149,43 @@ declare_syntax_cat wat_limits
 scoped syntax wat_u32     : wat_limits
 scoped syntax wat_u32 wat_u32 : wat_limits
 
-scoped syntax "[wat_limits|" wat_limits "]" : term
+scoped syntax ">>wat_limits|" wat_limits "<<" : term
 
 macro_rules
-| `([wat_limits| $n:wat_u32 ]) =>
-    `(Wasm.Syntax.Typ.Limit.mk [wat_u32| $n] .none)
-| `([wat_limits| $n:wat_u32 $m:wat_u32 ])  =>
-    `(Wasm.Syntax.Typ.Limit.mk [wat_u32| $n] (.some [wat_u32| $m]))
+| `(>>wat_limits| $n:wat_u32 <<) =>
+    `(Wasm.Syntax.Typ.Limit.mk >>wat_u32| $n<< .none)
+| `(>>wat_limits| $n:wat_u32 $m:wat_u32 <<)  =>
+    `(Wasm.Syntax.Typ.Limit.mk >>wat_u32| $n<< (.some >>wat_u32| $m<<))
 
 
 /- Memory Types -/
 declare_syntax_cat wat_memtype
 scoped syntax wat_limits : wat_memtype
 
-scoped syntax "[wat_memtype|" wat_memtype "]" : term
+scoped syntax ">>wat_memtype|" wat_memtype "<<" : term
 
 macro_rules
-| `([wat_memtype| $lim:wat_limits]) => `([wat_limits| $lim])
+| `(>>wat_memtype| $lim:wat_limits<<) => `(>>wat_limits| $lim<<)
 
 
 /- Table Types -/
 declare_syntax_cat wat_tabletype
 scoped syntax wat_limits wat_reftype : wat_tabletype
 
-scoped syntax "[wat_tabletype|" wat_tabletype "]" : term
+scoped syntax ">>wat_tabletype|" wat_tabletype "<<" : term
 
 macro_rules
-| `([wat_tabletype| $lim:wat_limits $et:wat_reftype]) =>
-    `(Typ.Table.mk [wat_limits| $lim] [wat_reftype| $et])
+| `(>>wat_tabletype| $lim:wat_limits $et:wat_reftype<<) =>
+    `(Typ.Table.mk >>wat_limits| $lim<< >>wat_reftype| $et<<)
 
 
 declare_syntax_cat wat_globaltype
 scoped syntax wat_valtype               : wat_globaltype
 scoped syntax "(" "mut" wat_valtype ")" : wat_globaltype
 
-scoped syntax "[wat_globaltype|" wat_globaltype "]" : term
+scoped syntax ">>wat_globaltype|" wat_globaltype "<<" : term
 
 macro_rules
-| `([wat_globaltype| $t:wat_valtype]) => `(Global.mk Mut.const [wat_valtype| $t])
-| `([wat_globaltype| (mut $t:wat_valtype)]) =>
-    `(Global.mk Mut.var [wat_valtype| $t])
+| `(>>wat_globaltype| $t:wat_valtype<<) => `(Global.mk Mut.const >>wat_valtype| $t<<)
+| `(>>wat_globaltype| (mut $t:wat_valtype)<<) =>
+    `(Global.mk Mut.var >>wat_valtype| $t<<)
