Wasm/Text/Notation/Value.lean
@@ -36,37 +36,37 @@ scoped syntax "↑" term:max : wat_i64
 scoped syntax wat_u64      : wat_i64
 scoped syntax wat_s64      : wat_i64
 
-scoped syntax "[wat_u32|" wat_u32 "]" : term
-scoped syntax "[wat_u64|" wat_u64 "]" : term
+scoped syntax ">>wat_u32|" wat_u32 "<<" : term
+scoped syntax ">>wat_u64|" wat_u64 "<<" : term
 
-scoped syntax "[wat_s32|" wat_s32 "]" : term
-scoped syntax "[wat_s33|" wat_s33 "]" : term
-scoped syntax "[wat_s64|" wat_s64 "]" : term
+scoped syntax ">>wat_s32|" wat_s32 "<<" : term
+scoped syntax ">>wat_s33|" wat_s33 "<<" : term
+scoped syntax ">>wat_s64|" wat_s64 "<<" : term
 
-scoped syntax "[wat_i32|" wat_i32 "]" : term
-scoped syntax "[wat_i64|" wat_i64 "]" : term
+scoped syntax ">>wat_i32|" wat_i32 "<<" : term
+scoped syntax ">>wat_i64|" wat_i64 "<<" : term
 
 macro_rules
-| `([wat_u32| $x:num])   => `(Unsigned.ofNat (n:=⟨32, by simp⟩) $x)
-| `([wat_u32| ↑$e:term]) => `($e)
-| `([wat_u64| $x:num])   => `(Unsigned.ofNat (n:=⟨64, by simp⟩) $x)
-| `([wat_u64| ↑$e:term]) => `($e)
+| `(>>wat_u32| $x:num<<)   => `(Unsigned.ofNat (n:=32) $x)
+| `(>>wat_u32| ↑$e:term<<) => `($e)
+| `(>>wat_u64| $x:num<<)   => `(Unsigned.ofNat (n:=64) $x)
+| `(>>wat_u64| ↑$e:term<<) => `($e)
 
-| `([wat_s32| $x:num])   => `(Signed.ofNat   (n:=⟨32, by simp⟩) $x)
-| `([wat_s32| ↑$e:term]) => `($e)
-| `([wat_s33| $x:num])   => `(Signed.ofNat   (n:=⟨33, by simp⟩) $x)
-| `([wat_s33| ↑$e:term]) => `($e)
-| `([wat_s64| $x:num])   => `(Signed.ofNat   (n:=⟨64, by simp⟩) $x)
-| `([wat_s64| ↑$e:term]) => `($e)
+| `(>>wat_s32| $x:num<<)   => `(Signed.ofNat   (n:=32) $x)
+| `(>>wat_s32| ↑$e:term<<) => `($e)
+| `(>>wat_s33| $x:num<<)   => `(Signed.ofNat   (n:=33) $x)
+| `(>>wat_s33| ↑$e:term<<) => `($e)
+| `(>>wat_s64| $x:num<<)   => `(Signed.ofNat   (n:=64) $x)
+| `(>>wat_s64| ↑$e:term<<) => `($e)
 
-| `([wat_i32| $x:num])     => `(Unsigned.ofNat (n:=⟨32, by simp⟩) $x)
-| `([wat_i32| ↑$e:term])   => `($e)
-| `([wat_i32| $x:wat_u32]) => `([wat_u32| $x])
-| `([wat_i32| $x:wat_s32]) => `([wat_s32| $x])
-| `([wat_i64| $x:num])     => `(Unsigned.ofNat (n:=⟨64, by simp⟩) $x)
-| `([wat_i64| ↑$e:term])   => `($e)
-| `([wat_i64| $x:wat_u64]) => `([wat_u64| $x])
-| `([wat_i64| $x:wat_s64]) => `([wat_s64| $x])
+| `(>>wat_i32| $x:num<<)     => `(Unsigned.ofNat (n:=32) $x)
+| `(>>wat_i32| ↑$e:term<<)   => `($e)
+| `(>>wat_i32| $x:wat_u32<<) => `(>>wat_u32| $x<<)
+| `(>>wat_i32| $x:wat_s32<<) => `(>>wat_s32| $x<<)
+| `(>>wat_i64| $x:num<<)     => `(Unsigned.ofNat (n:=64) $x)
+| `(>>wat_i64| ↑$e:term<<)   => `($e)
+| `(>>wat_i64| $x:wat_u64<<) => `(>>wat_u64| $x<<)
+| `(>>wat_i64| $x:wat_s64<<) => `(>>wat_s64| $x<<)
 
 
 declare_syntax_cat wat_ident
@@ -75,19 +75,17 @@ scoped syntax ident        : wat_ident
 scoped syntax "↑" term:max : wat_ident
 scoped syntax wat_ident ?  : wat_ident?
 
-scoped syntax "[wat_ident_str|" ident "]" : term
-scoped syntax "[wat_ident|" wat_ident "]" : term
-scoped syntax "[wat_ident?|" wat_ident? "]" :term
+scoped syntax ">>wat_ident_str|" ident "<<" : term
+scoped syntax ">>wat_ident|" wat_ident "<<" : term
+scoped syntax ">>wat_ident?|" wat_ident? "<<" :term
 
 /- TODO: identifiers in WAT should be preceded by a `$` but this clashes with -/
 macro_rules
-| `([wat_ident_str| $id:ident]) =>
-  return Lean.Syntax.mkStrLit id.getId.toString
-| `([wat_ident| $id:ident]) =>
-  `(Ident.mk [wat_ident_str| $id] sorry sorry)
-| `([wat_ident| ↑$e]) => `($e)
-| `([wat_ident?| $id:wat_ident]) => `(.some [wat_ident| $id])
-| `([wat_ident?| ]) => `(.none)
+| `(>>wat_ident_str| $id:ident<<) => return Lean.Syntax.mkStrLit id.getId.toString
+| `(>>wat_ident| $id:ident<<) => `(Ident.mk >>wat_ident_str| $id<< sorry sorry)
+| `(>>wat_ident| ↑$e<<) => `($e)
+| `(>>wat_ident?| $id:wat_ident<<) => `(.some >>wat_ident| $id<<)
+| `(>>wat_ident?| <<) => `(.none)
 
 
 declare_syntax_cat wat_value
@@ -99,12 +97,12 @@ scoped syntax wat_ident    : wat_value
 scoped syntax str          : wat_value
 scoped syntax "↑" term:max : wat_value
 
-scoped syntax "[wat_value|" wat_value "]" : term
+scoped syntax ">>wat_value|" wat_value "<<" : term
 
 macro_rules
-| `([wat_value| $n:wat_u32    ]) => `([wat_u32| $n])
-| `([wat_value| $n:wat_u64    ]) => `([wat_u64| $n])
-| `([wat_value| $n:wat_s32    ]) => `([wat_s32| $n])
-| `([wat_value| $n:wat_s64    ]) => `([wat_s64| $n])
-| `([wat_value| $id:wat_ident ]) => `([wat_ident| $id])
-| `([wat_value| ↑$e ])           => `($e)
+| `(>>wat_value| $n:wat_u32    <<) => `(>>wat_u32| $n<<)
+| `(>>wat_value| $n:wat_u64    <<) => `(>>wat_u64| $n<<)
+| `(>>wat_value| $n:wat_s32    <<) => `(>>wat_s32| $n<<)
+| `(>>wat_value| $n:wat_s64    <<) => `(>>wat_s64| $n<<)
+| `(>>wat_value| $id:wat_ident <<) => `(>>wat_ident| $id<<)
+| `(>>wat_value| ↑$e <<)           => `($e)
